Progress on wpr lemmas

src/base/post_crash_modality.v
@@ -1,6 +1,7 @@
 (* In this file we define the post crash modality for the base logic. *)
 From Coq Require Import QArith Qcanon.
 From iris.algebra Require Import agree.
+From iris.bi Require Import fractional.
 From iris.proofmode Require Import reduction monpred tactics.
 
 From Perennial.program_logic Require Export crash_lang.
@@ -12,6 +13,14 @@ From self.base Require Import primitive_laws.
 
 Set Default Proof Using "Type".
 
+Lemma foo qp prf : (* Upstream *)
+  mk_Qp (Qp_to_Qc qp) prf = qp.
+Proof. by apply Qp_to_Qc_inj_iff. Qed.
+
+(* upstream *)
+Lemma Qp_to_Qc_add p q : (Qp_to_Qc p + Qp_to_Qc q = Qp_to_Qc (p + q))%Qc.
+Proof. by destruct p, q. Qed.
+
 (** This definition captures the resources and knowledge you gain _after_ a
 crash if you own a points-to predicate _prior to_ a crash. *)
 Definition mapsto_post_crash {Σ} (hG : nvmBaseG Σ) ℓ q (hist : history) : iProp Σ :=
@@ -21,11 +30,106 @@ Definition mapsto_post_crash {Σ} (hG : nvmBaseG Σ) ℓ q (hist : history) : iP
             ∃ RV, ⌜msg.(msg_persisted_after_view) ⊑ RV⌝ ∗ recovered RV) ∨
   (∀ t, ¬ (recovered {[ ℓ := MaxNat t ]})).
 
-Definition if_non_zero {Σ} (q : Qc) (P : Qp → iProp Σ) : iProp Σ :=
-  match (decide (0 < q)%Qc) with
-    left prf => P (mk_Qp q prf)
-  | right prf => ⌜q = 0⌝
-  end.
+Instance fractional_mapsto_post_crash {Σ : gFunctors} hG' ℓ hist : Fractional (λ p : Qp, mapsto_post_crash (Σ := Σ) hG' ℓ p hist).
+Proof.
+  rewrite /Fractional.
+  iIntros (p q).
+  rewrite /mapsto_post_crash.
+  iSplit.
+  - admit.
+  - admit.
+Admitted.
+
+Section if_non_zero.
+  Context {Σ : gFunctors}.
+  Implicit Types (P : Qp → iProp Σ).
+
+  Definition if_non_zero (q : Qc) P : iProp Σ :=
+    match (decide (0 < q)%Qc) with
+      left prf => P (mk_Qp q prf)
+    | right prf => ⌜q = 0%Qc⌝
+    end.
+
+  Lemma if_non_zero_cases q P :
+    if_non_zero q P ⊣⊢ ⌜q = 0%Qc⌝ ∨ ∃ qp, ⌜(0 < q)%Qc⌝ ∗ ⌜q = Qp_to_Qc qp⌝ ∗ P qp.
+  Proof.
+    rewrite /if_non_zero.
+    iSplit.
+    - destruct (decide (0 < q)%Qc).
+      * iIntros. iRight. iExists _. iFrame. done.
+      * auto.
+    - iIntros "[->|H]"; first done.
+      iDestruct "H" as (qp) "(% & % & ?)".
+      rewrite decide_left. simplify_eq. rewrite foo. iFrame.
+  Qed.
+
+  Lemma if_non_zero_ge_0 q P : if_non_zero q P -∗ ⌜(0 ≤ q)%Qc⌝.
+  Proof.
+    rewrite /if_non_zero. destruct (decide (0 < q)%Qc).
+    - iIntros. iPureIntro. apply Qclt_le_weak. done.
+    - iIntros (->). done.
+  Qed.
+
+  Lemma if_non_zero_add (P : Qp → iProp Σ) `{!Fractional P} p q :
+    ⊢ P p -∗ if_non_zero q P -∗ if_non_zero (q + (Qp_to_Qc p)) P.
+  Proof.
+    iIntros "P P'".
+    iApply if_non_zero_cases. iRight.
+    iDestruct (if_non_zero_cases with "P'") as "[-> | H]".
+    - iExists _. iFrame. iPureIntro.
+      rewrite Qcplus_0_l.
+      split; last done. apply Qp_prf.
+    - iDestruct "H" as (qp) "(%gt & %eq & P')".
+      iExists (p + qp)%Qp.
+      rewrite (fractional p qp).
+      iFrame.
+      (* The rest is just reasoning with Qp arithemitic. *)
+  Admitted.
+
+  Lemma if_non_zero_subtract (P : Qp → iProp Σ) `{!Fractional P} p q :
+    (Qp_to_Qc p ≤ q)%Qc →
+    ⊢ if_non_zero q P -∗ if_non_zero (q - Qp_to_Qc p) P ∗ P p.
+  Proof.
+    iIntros (le) "P".
+    iDestruct (if_non_zero_cases with "P") as "[-> | H]".
+    - exfalso.
+      apply Qcle_not_lt in le.
+      apply (le (Qp_prf _)).
+    - iDestruct "H" as (qp) "(%gt & %eq & P')".
+      rewrite /if_non_zero.
+      destruct (decide (0 < q - Qp_to_Qc p)%Qc).
+      * rewrite -fractional.
+        eassert (qp = _) as ->; last iFrame.
+        apply Qp_to_Qc_inj_iff.
+        rewrite -Qp_to_Qc_add.
+        simpl.
+        rewrite /Qcminus.
+        rewrite -Qcplus_assoc.
+        rewrite (Qcplus_comm _ (Qp_to_Qc _)).
+        rewrite Qcplus_opp_r.
+        rewrite Qcplus_0_r.
+        done.
+      * admit.
+  Admitted.
+
+  Lemma if_non_zero_exchange_1 (q1 q2 : Qc) p (P Q : Qp → iProp Σ) `{!Fractional P, !Fractional Q}:
+    (Qp_to_Qc p ≤ q2)%Qc →
+    P p ∗ if_non_zero q1 P ∗ if_non_zero q2 Q ⊢
+    if_non_zero (q1 + Qp_to_Qc p)  P ∗ if_non_zero (q2 - Qp_to_Qc p) Q ∗ Q p.
+  Proof.
+    iIntros (le) "(P & ZP & ZQ)".
+    iDestruct (if_non_zero_subtract with "ZQ") as "[$ $]"; first done.
+    iApply (if_non_zero_add with "P [$]").
+  Qed.
+
+  Lemma mk_Qp_1 prf : mk_Qp 1 prf = 1%Qp.
+  Proof. apply Qp_to_Qc_inj_iff. simpl. by rewrite Z2Qc_inj_1. Qed.
+
+  Lemma if_non_zero_1 (P : Qp → iProp Σ) :
+    if_non_zero 1%Qc P = P 1%Qp.
+  Proof. rewrite /if_non_zero. simpl. by rewrite mk_Qp_1. Qed.
+
+End if_non_zero.
 
 (* Note: The odd [let]s below are to manipulate the type class instance search. *)
 
@@ -52,12 +156,55 @@ Proof.
   iAssert (⌜σ__old !! ℓ = Some hist⌝)%I as %elemof.
   { iApply "look". iFrame. }
   iDestruct (big_sepM_lookup_acc with "map") as "[elm reIns]"; first done.
-  iDestruct "elm" as (q' p) "(oldPts & new & %eq)".
-  (* { iDestruct (mapsto_ne with "pts pts'") as %hi. done. } *)
-  (* We reinsert. *)
-  (* iDestruct ("reIns" with "[$pts]") as "map". *)
-  (* iFrame "#∗". *)
-Admitted.
+  iDestruct "elm" as (qOld qNew) "(oldPts & new & %eq)".
+
+  iAssert (⌜Qp_to_Qc q ≤ qNew⌝)%Qc%I as %test.
+  {
+    iDestruct (if_non_zero_cases with "oldPts") as "[-> | H]".
+    - rewrite Qcplus_0_l in eq.
+      rewrite eq.
+      iDestruct (mapsto_valid with "pts") as "%le".
+      iPureIntro.
+      setoid_rewrite dfrac_valid_own in le.
+      apply Qp_to_Qc_inj_le in le.
+      apply le.
+    - iDestruct "H" as (qp) "(%gt & %eq' & P')".
+      iDestruct (mapsto_valid_2 with "pts P'") as "[%le _]".
+      iPureIntro.
+      rewrite dfrac_op_own in le.
+      setoid_rewrite dfrac_valid_own in le.
+      apply Qp_to_Qc_inj_le in le.
+      rewrite -Qp_to_Qc_add in le.
+      rewrite -eq' in le.
+      simpl in le.
+      assert (qNew = 1 - qOld)%Qc as ->.
+      { rewrite -eq.
+        rewrite Qcplus_comm.
+        rewrite /Qcminus.
+        rewrite -Qcplus_assoc.
+        rewrite Qcplus_opp_r.
+        by rewrite Qcplus_0_r. }
+      rewrite Qcplus_le_mono_r.
+      etrans; first apply le.
+      rewrite /Qcminus.
+      rewrite -Qcplus_assoc.
+      rewrite (Qcplus_comm _ qOld).
+      rewrite Qcplus_opp_r.
+      done. }
+  iDestruct (if_non_zero_exchange_1 with "[$oldPts $new $pts]") as "(? & ? & $)".
+  { done. }
+  iFrame.
+  iApply "reIns".
+  iExists _, _. iFrame. iPureIntro.
+  rewrite Qcplus_assoc.
+  rewrite (Qcplus_comm _ qNew).
+  rewrite -Qcplus_assoc.
+  rewrite -Qcplus_assoc.
+  rewrite (Qcplus_opp_r (Qp_to_Qc q)).
+  rewrite Qcplus_0_r.
+  rewrite Qcplus_comm.
+  done.
+Qed.
 
 Definition persisted_impl {Σ} hG hG' : iProp Σ :=
   □ ∀ V, persisted (hG := hG) V -∗ persisted (hG := hG') ∅ ∗
